src/Imp/Frontend/Parser/PEG/Parser.hs
@@ -1,0 +1,3 @@
+module Imp.Frontend.Parser.PEG.Parser where
+
+import Parser.PEG.ParsingExp 
