src/Imp/Frontend/Parser/Recursive/Parser.hs
@@ -1,0 +1,187 @@
+module Imp.Frontend.Parser.Recursive.Parser where 
+
+{-
+ - Recursive descendent parser 
+ - This is an scannerless parser. 
+ - -}
+
+import Parser.Recursive.SimpleCombinators
+import Imp.Syntax.Syntax
+
+-- top level parsing function 
+
+impParser :: String -> Either String Program
+impParser s 
+  = case runParser programParser s of 
+      [] -> Left "Parser error"
+      ((r,_) : _) -> Right r
+
+-- main program parser 
+
+programParser :: Parser Char Program
+programParser 
+  = Program <$> blockParser
+
+-- parser for statements 
+ 
+stmtParser :: Parser Char Stmt 
+stmtParser 
+  = choice [
+             skipParser
+           , varDeclParser  
+           , assignParser
+           , ifParser 
+           , printParser 
+           , readParser 
+           ]
+
+-- skip statement 
+
+skipParser :: Parser Char Stmt 
+skipParser 
+  = Skip <$ (stringToken "skip") <* (stringToken ";")
+
+-- variable declaration 
+
+varDeclParser :: Parser Char Stmt
+varDeclParser
+  = f <$> tyParser <*> varParser <*> initParser <*> semi 
+    where 
+      f t v i _ = Def t v i
+
+-- variable 
+
+varParser :: Parser Char Var 
+varParser = Var <$> identifier
+
+-- type 
+
+tyParser :: Parser Char Ty 
+tyParser = intParser <|> tboolParser 
+
+intParser :: Parser Char Ty 
+intParser = TInt <$ (stringToken "int")
+
+tboolParser :: Parser Char Ty 
+tboolParser = TBool <$ (stringToken "bool")
+
+-- initialization 
+
+initParser :: Parser Char (Maybe Exp)
+initParser = (Just <$> rhsParser) <|> pure Nothing 
+
+rhsParser :: Parser Char Exp
+rhsParser 
+  = f <$> stringToken ":=" <*> expParser 
+    where
+      f _ e = e
+
+-- assignment 
+
+assignParser :: Parser Char Stmt 
+assignParser 
+  = f <$> varParser <*> rhsParser <*> semi 
+    where 
+      f v e _ = v := e
+
+
+-- blocks 
+
+blockParser :: Parser Char Block
+blockParser 
+  = Block <$> braces (greedy stmtParser)
+
+-- if statement 
+
+ifParser :: Parser Char Stmt
+ifParser 
+  = f <$> stringToken "if"   <*> 
+          expParser          <*> 
+          stringToken "then" <*> 
+          blockParser        <*> 
+          stringToken "else" <*> 
+          blockParser
+    where 
+      f _ b _ bt _ be = If b bt be
+
+-- print statement 
+
+printParser :: Parser Char Stmt 
+printParser 
+  = Print <$> expParser 
+
+-- read statement 
+
+readParser :: Parser Char Stmt 
+readParser 
+  = SRead <$> varParser
+
+-- while statement 
+
+whileParser :: Parser Char Stmt 
+whileParser 
+  = f <$> stringToken "while" <*> expParser <*> blockParser
+    where 
+      f _ e b = While e b
+
+-- values 
+
+valueParser :: Parser Char Value 
+valueParser = vintParser <|> vboolParser 
+
+vintParser :: Parser Char Value
+vintParser = EInt <$> integer 
+
+vboolParser :: Parser Char Value 
+vboolParser = EBool <$> boolParser 
+  where 
+    boolParser = trueParser <|> falseParser 
+    trueParser = True <$ stringToken "true"
+    falseParser = False <$ stringToken "false"
+
+-- expressions.
+
+expParser :: Parser Char Exp 
+expParser = andExpParser
+
+andExpParser :: Parser Char Exp
+andExpParser 
+  = chainl relExpParser andop 
+    where 
+      andop = (:&:) <$ stringToken "&&"
+
+relExpParser :: Parser Char Exp
+relExpParser 
+  = chainr plusExpParser relop  
+    where 
+      relop = eqp <|> ltp
+      eqp = (:==:) <$ stringToken "=="
+      ltp = (:<:) <$ stringToken "<"
+
+plusExpParser :: Parser Char Exp
+plusExpParser 
+  = chainl mulExpParser plusop  
+    where 
+      plusop = plusp <|> minusp
+      plusp = (:+:) <$ stringToken "+"
+      minusp = (:-:) <$ stringToken "-"
+
+mulExpParser :: Parser Char Exp
+mulExpParser 
+  = chainl notExpParser mulop  
+    where 
+      mulop = timesp <|> divp
+      timesp = (:*:) <$ stringToken "*"
+      divp = (:/:) <$ stringToken "/"
+
+notExpParser :: Parser Char Exp
+notExpParser 
+  = (const ENot <$> (stringToken "!")) `option` id <*> factorParser 
+
+factorParser :: Parser Char Exp
+factorParser 
+  = choice [ EValue <$> valueParser
+           , EVar <$> varParser
+           , parens expParser 
+           ]
+    
