lean/Imp/Derived.lean
@@ -1,0 +1,76 @@
+import Mathlib.Data.Nat.Defs 
+import Mathlib.Tactic.Basic 
+
+import Aesop 
+
+import Imp.Hoare
+import Imp.Syntax
+import Imp.Interpreter 
+import Imp.Semantics 
+
+-- some derived rules for Hoare logic 
+
+theorem Consequence_left (P') {P Q s} 
+  : {* P *}(s) {* Q *} → 
+    (∀ st, P' st → P st) → 
+    {* P' *}(s) {* Q *} := by 
+    intros H1 H2
+    apply Consequence_rule 
+    exact H1 
+    exact H2 
+    intros _st H3 ; exact H3 
+
+theorem Consequence_right (Q){P Q' s}
+  : {* P *}(s) {* Q *} → 
+    (∀ st, Q st → Q' st) → 
+    {* P *} (s) {* Q' *} := by 
+    
+    intros H1 H2 
+    apply Consequence_rule 
+    exact H1 
+    intros _ H1 ; exact H1 
+    exact H2 
+
+theorem Skip_rule' {P Q} 
+  : (∀ st, P st → Q st) → 
+    {* P *} (Stmt.Skip) {* Q *} := by 
+    intros H1 
+    apply Consequence_right 
+    apply Skip_rule 
+    assumption 
+
+theorem Assign_rule' {P Q x a} 
+  : (∀ st, P st → Q (x |-> (evalExp a st) ; st)) → 
+    {* P *}(Stmt.Assign x a) {* Q *} := by 
+    intros H env env' Hp HEval 
+    rcases HEval 
+    rename_i v Heq 
+    specialize H env 
+    rw [Heq] at H 
+    apply H 
+    exact Hp 
+
+theorem Seq_rule' {P Q R s1 s2} 
+  : {* Q *} (s2) {* R *} → 
+    {* P *} (s1) {* Q *} → 
+    {* P *} (Stmt.Seq s1 s2) {* R *} := by 
+    intros H1 H2 env env' Hp Heval 
+    rcases Heval 
+    rename_i env1 H4 H5  
+    apply H1 <;> try assumption 
+    apply H2 <;> try assumption 
+
+theorem While_rule' {P Q a s}(I)
+  (H1 : {* I .&. True(a) *} (s) {* I *}) 
+  (H2 : (∀ st, P st → I st)) 
+  (H3 : ∀ st, evalExp a st = 0 → I st → Q st) : 
+    {* P *}(Stmt.While a s){* Q *} := by 
+    apply Consequence_rule
+    apply While_rule
+    apply H1 
+    assumption
+    intros st H4
+    specialize H3 st 
+    simp [assert_and] at H4
+    rcases H4 with ⟨ H41 , H42 ⟩ 
+    apply H3 <;> try assumption 
