lean/Imp/Sequences.lean
@@ -1,0 +1,36 @@
+import Mathlib.Tactic 
+import Aesop 
+
+section SEQUENCES
+
+  -- reflexive and transitive closure 
+  
+  inductive star {A : Type}{R : A → A → Prop} : A → A → Prop where 
+  | srefl x : star x x 
+  | sstep x y z : R x y → star y z → star x z
+
+  theorem starone {A : Type}{R : A → A → Prop}{x y : A} 
+    : R x y → @star A R x y := by 
+      intros H
+      apply star.sstep 
+      exact H 
+      apply star.srefl 
+
+  lemma startrans {A : Type}{R : A → A → Prop}{x y} 
+    : @star A R x y → ∀ z, @star A R y z → @star A R x z := by 
+      intros H1
+      induction H1 
+      · 
+        intros z H2
+        aesop 
+      · 
+        intros z H2
+        rename_i H3 _H4 IH
+        apply star.sstep 
+        exact H3 
+        apply IH 
+        assumption 
+
+   
+
+end SEQUENCES
