lean/Imp/Swap.lean
@@ -1,0 +1,28 @@
+import Imp.Syntax 
+import Imp.Hoare 
+import Imp.Derived
+
+def swap : Stmt := 
+  {imp| 
+    tmp := x :;: 
+    x := y :;: 
+    y := tmp 
+  }
+
+theorem swap_correct (a b : ℕ) 
+  : {* λ st => st "x" = a ∧ st "y" = b *}
+      (swap)
+    {* λ st => st "x" = b ∧ st "y" = a *} := by 
+    apply Seq_rule'
+    apply Seq_rule' 
+    apply Assign_rule
+    apply Assign_rule
+    apply Assign_rule'
+    simp [assertion_sub, updateEnv, evalExp]
+    intros st H1 H2
+    constructor 
+    · 
+      sorry 
+    · 
+      sorry 
+     
